\begin{activity} \label{A:9.4.3}  Let $\vu$ and $\vv$ be vectors in $\R^3$ and let $c$ be a scalar. Use (\ref{eq:9.4.cp_anticomm}) and (\ref{eq:9.4.cp_scalar}) to show that
\[\vu \times (c\vv) = c(\vu \times \vv).\]
\end{activity}
\begin{smallhint}

\end{smallhint}
\begin{bighint}

\end{bighint}
\begin{activitySolution}
By (\ref{eq:9.4.cp_anticomm}) we have 
\[\vu \times (c\vv) = -((c\vv) \times \vu).\]
Property (\ref{eq:9.4.cp_scalar}) gives us 
\[\vu \times (c\vv) = -(c)(\vv \times \vu).\]
Applying (\ref{eq:9.4.cp_anticomm}) again shows that
\[\vu \times (c\vv) = -(c)(-\vu \times \vv) = c(\vu \times \vv).\]
\end{activitySolution}
\aftera
